theories/CodegenWasm/toplevel.v
@@ -1,0 +1,22 @@
+From Wasm Require Import datatypes.
+
+From Coq Require Import ZArith List.
+Require Import Common.Common Common.compM Common.Pipeline_utils.
+Require Import LambdaANF.cps LambdaANF.cps_show CodegenWasm.LambdaANF_to_Wasm.
+
+Require Import ExtLib.Structures.Monad.
+Import MonadNotation.
+
+Definition LambdaANF_to_Wasm_Wrapper (prims : list (kername * string * bool * nat * positive)) (args : nat) (t : toplevel.LambdaANF_FullTerm) : error module * string :=
+  let '(_, pr_env, cenv, ctag, itag, nenv, fenv, _, prog) := t in
+  match LambdaANF_to_Wasm nenv cenv prog with
+  | Ret res => let '(module, _, _) := res in (Ret module, "")
+  | Err err => (Err err, "")
+  end.
+
+Definition compile_LambdaANF_to_Wasm (prims : list (kername * string * bool * nat * positive)) : CertiCoqTrans toplevel.LambdaANF_FullTerm module :=
+  fun s =>
+    debug_msg "Translating from LambdaANF to Wasm" ;;
+    opts <- get_options ;;
+    let args := c_args opts in
+    LiftErrorLogCertiCoqTrans "CodegenWasm" (LambdaANF_to_Wasm_Wrapper prims args) s.
