theories/Compiler/pipeline.v
@@ -1,6 +1,6 @@
 From Wasm Require Import binary_format_printer.
 
-Require Export LambdaBoxMut.toplevel LambdaBoxLocal.toplevel LambdaANF.toplevel Codegen.toplevel CodegenWASM.toplevel.
+Require Export LambdaBoxMut.toplevel LambdaBoxLocal.toplevel LambdaANF.toplevel Codegen.toplevel CodegenWasm.toplevel.
 Require Import compcert.lib.Maps.
 Require Import ZArith.
 Require Import Common.Common Common.compM Common.Pipeline_utils.
@@ -133,12 +133,12 @@ Definition pipeline (p : Template.Ast.Env.program) :=
  *)  p <- CertiCoq_pipeline next_id prs false p ;;
   compile_Clight prs p.
 
-Definition pipeline_WASM (p : Template.Ast.Env.program) :=
+Definition pipeline_Wasm (p : Template.Ast.Env.program) :=
   let genv := fst p in
   '(prs, next_id) <- register_prims next_id genv.(Ast.Env.declarations) ;;
 (*   p <- erase_PCUIC p ;;
  *)  p <- CertiCoq_pipeline next_id prs false p ;;
-     compile_LambdaANF_to_WASM prs p.
+     compile_LambdaANF_to_Wasm prs p.
 
 Definition default_opts : Options :=
   {| direct := false;
@@ -201,9 +201,9 @@ Definition show_IR (opts : Options) (p : Template.Ast.Env.program) : (error stri
   end.
 
 
-(** * For compiling lambda_ANF to WASM *)
-Definition compile_WASM (opts : Options) (p : Template.Ast.Env.program) : (error string * string) :=
-let (perr, log) := run_pipeline _ _ opts p pipeline_WASM in
+(** * For compiling lambda_ANF to Wasm *)
+Definition compile_Wasm (opts : Options) (p : Template.Ast.Env.program) : (error string * string) :=
+let (perr, log) := run_pipeline _ _ opts p pipeline_Wasm in
   match perr with
   | Ret p => (Ret (String.parse (binary_of_module p)), log)
   | Err s => (Err s, log)
