theories/Extraction/extraction.v
@@ -105,7 +105,7 @@ Separate Extraction
          Glue.ffi.generate_ffi
          cps.M.elements
          Compiler.pipeline.show_IR
-         Compiler.pipeline.compile_WASM.
+         Compiler.pipeline.compile_Wasm.
 
 Recursive Extraction Library Ascii.
 Recursive Extraction Library BinPos.
